backend/Linear_old.v
@@ -17,8 +17,8 @@
     instructions with explicit labels and ``goto'' instructions. *)
 
 Require Import Coqlib.
-Require Import AST Integers Values Memory Events Globalenvs Smallstep.
-Require Import Op Locations LTL Conventions.
+Require Import AST_old Integers Values_old Memory_old Events_old Globalenvs_old Smallstep_old.
+Require Import Op_old Locations_old LTL_old Conventions_old.
 
 (** * Abstract syntax *)
 
@@ -47,9 +47,9 @@ Record function: Type := mkfunction {
   fn_code: code
 }.
 
-Definition fundef := AST.fundef function.
+Definition fundef := AST_old.fundef function.
 
-Definition program := AST.program fundef unit.
+Definition program := AST_old.program fundef unit.
 
 Definition funsig (fd: fundef) :=
   match fd with
@@ -89,17 +89,7 @@ Fixpoint find_label (lbl: label) (c: code) {struct c} : option code :=
   | i1 :: il => if is_label lbl i1 then Some il else find_label lbl il
   end.
 
-(*SACC:*)
-Section STACK_WRAPPER.
-
-(*SACC:*)
-Variable fn_stack_requirements : ident -> Z.
-
-Section RELSEM.
-
-Variable ge: genv.
-
-Definition find_function (ros: mreg + ident) (rs: locset) : option fundef :=
+Definition find_function (ge: genv) (ros: mreg + ident) (rs: locset) : option fundef :=
   match ros with
   | inl r => Genv.find_funct ge (rs (R r))
   | inr symb =>
@@ -107,13 +97,6 @@ Definition find_function (ros: mreg + ident) (rs: locset) : option fundef :=
       | None => None
       | Some b => Genv.find_funct_ptr ge b
       end
-  end.
-
-(*SACC:*)
-Definition ros_is_function (ros: mreg + ident) (rs: locset) (i: ident) : Prop :=
-  match ros with
-  | inl r => exists b o, rs (R r) = Vptr b o /\ Genv.find_symbol ge i = Some b
-  | inr symb => i = symb
   end.
 
 (** Linear execution states. *)
@@ -126,7 +109,7 @@ Inductive stackframe: Type :=
              (c: code),            (**r program point in calling function *)
       stackframe.
 
-Inductive state: Type :=
+Inductive state `{memory_model_ops: Mem.MemoryModelOps}: Type :=
   | State:
       forall (stack: list stackframe) (**r call stack *)
              (f: function)            (**r function currently executing *)
@@ -139,8 +122,7 @@ Inductive state: Type :=
       forall (stack: list stackframe) (**r call stack *)
              (f: fundef)              (**r function to call *)
              (rs: locset)             (**r location state at point of call *)
-             (m: mem)                 (**r memory state *)
-             (sz: Z),                 (**r stack size requirement for callee *)
+             (m: mem) (sz: Z),                (**r memory state *)
       state
   | Returnstate:
       forall (stack: list stackframe) (**r call stack *)
@@ -148,12 +130,30 @@ Inductive state: Type :=
              (m: mem),                (**r memory state *)
       state.
 
+Section WITHEXTERNALCALLSOPS.
+Context `{external_calls_prf: ExternalCalls}.
+
+Variable fn_stack_requirements: ident -> Z.
+
+Section RELSEM.
+
 (** [parent_locset cs] returns the mapping of values for locations
   of the caller function. *)
+
+Variable parent_lm: locset.
+
 Definition parent_locset (stack: list stackframe) : locset :=
   match stack with
-  | nil => Locmap.init Vundef
+  | nil => parent_lm
   | Stackframe f sp ls c :: stack' => ls
+  end.
+
+Variable ge: genv.
+
+Definition ros_is_function (ros: mreg + ident) (rs: locset) (i: ident) : Prop :=
+  match ros with
+  | inl r => exists b o, rs (R r) = Vptr b o /\ Genv.find_symbol ge i = Some b
+  | inr symb => i = symb
   end.
 
 Inductive step: state -> trace -> state -> Prop :=
@@ -188,30 +188,29 @@ Inductive step: state -> trace -> state -> Prop :=
       step (State s f sp (Lstore chunk addr args src :: b) rs m)
         E0 (State s f sp b rs' m')
   | exec_Lcall:
-      forall s f sp sig ros b rs m f' (*SACC:*)fid
-      ((*SACC:*)IFI: ros_is_function ros rs fid),
-      find_function ros rs = Some f' ->
+      forall s f sp sig ros b rs m f' id (IFI: ros_is_function ros rs id) ,
+      find_function ge ros rs = Some f' ->
       sig = funsig f' ->
       step (State s f sp (Lcall sig ros :: b) rs m)
-        E0 (Callstate (Stackframe f sp rs b:: s) f' rs ((*SACC:*)Mem.push_new_stage m) ((*SACC:*)fn_stack_requirements fid))
+        E0 (Callstate (Stackframe f sp rs b:: s) f' rs (Mem.push_new_stage m) (fn_stack_requirements id))
   | exec_Ltailcall:
-      forall s f stk sig ros b rs m rs' f' m' (*SACC:*)m'' (*SACC:*)fid
-      ((*SACC:*)IFI: ros_is_function ros rs' fid),
+      forall s f stk sig ros b rs m rs' f' m' m'' id (IFI: ros_is_function ros rs' id),
       rs' = return_regs (parent_locset s) rs ->
-      find_function ros rs' = Some f' ->
+      find_function ge ros rs' = Some f' ->
       sig = funsig f' ->
       Mem.free m stk 0 f.(fn_stacksize) = Some m' ->
-  (*SACC:*)Mem.tailcall_stage m' = Some m'' ->
+      Mem.tailcall_stage m' = Some m'' ->
       step (State s f (Vptr stk Ptrofs.zero) (Ltailcall sig ros :: b) rs m)
-        E0 (Callstate s f' rs' (*SACC:*)m'' ((*SACC:*)fn_stack_requirements fid))
+        E0 (Callstate s f' rs' m'' (fn_stack_requirements id))
   | exec_Lbuiltin:
-      forall s f sp rs m ef args res b vargs t vres rs' m' (*SACC:*)m'',
+      forall s f sp rs m ef args res b vargs t vres rs' m' m'',
       eval_builtin_args ge rs sp m args vargs ->
-      external_call ef ge vargs ((*SACC:*)Mem.push_new_stage m) t vres m' ->
-  (*SACC:*)Mem.unrecord_stack_block m' = Some m'' ->
+      external_call ef ge vargs (Mem.push_new_stage m) t vres m' ->
+      Mem.unrecord_stack_block m' = Some m'' ->
       rs' = Locmap.setres res vres (undef_regs (destroyed_by_builtin ef) rs) ->
-      step (State s f sp (Lbuiltin ef args res :: b) rs m)
-         t (State s f sp b rs' (*SACC:*)m'')
+      forall BUILTIN_ENABLED : builtin_enabled ef,
+        step (State s f sp (Lbuiltin ef args res :: b) rs m)
+             t (State s f sp b rs' m'')
   | exec_Llabel:
       forall s f sp lbl b rs m,
       step (State s f sp (Llabel lbl :: b) rs m)
@@ -244,40 +243,193 @@ Inductive step: state -> trace -> state -> Prop :=
         E0 (State s f sp b' rs' m)
   | exec_Lreturn:
       forall s f stk b rs m m',
-      Mem.free m stk 0 f.(fn_stacksize) = Some m' ->
+        Mem.free m stk 0 f.(fn_stacksize) = Some m' ->
       step (State s f (Vptr stk Ptrofs.zero) (Lreturn :: b) rs m)
         E0 (Returnstate s (return_regs (parent_locset s) rs) m')
   | exec_function_internal:
-      forall s f rs m rs' m' stk (*SACC:*)m'' (*SACC:*)sz,
-      Mem.alloc m 0 f.(fn_stacksize) = (m', stk) ->
-  (*SACC:*)Mem.record_stack_blocks m' (make_singleton_frame_adt stk (fn_stacksize f) sz) = Some m'' ->
+      forall s f rs m rs' m' stk m'' sz,
+        Mem.alloc m 0 f.(fn_stacksize) = (m', stk) ->
+        Mem.record_stack_blocks m' (make_singleton_frame_adt stk (fn_stacksize f) sz) = Some m'' ->
       rs' = undef_regs destroyed_at_function_entry (call_regs rs) ->
-      step (Callstate s (Internal f) rs m (*SACC:*)sz)
-        E0 (State s f (Vptr stk Ptrofs.zero) f.(fn_code) rs' (*SACC:*)m'')
+      step (Callstate s (Internal f) rs m sz)
+        E0 (State s f (Vptr stk Ptrofs.zero) f.(fn_code) rs' m'')
   | exec_function_external:
-      forall s ef args res rs1 rs2 m t m' (*SACC:*)sz,
+      forall s ef args res rs1 rs2 m t m' sz,
       args = map (fun p => Locmap.getpair p rs1) (loc_arguments (ef_sig ef)) ->
       external_call ef ge args m t res m' ->
-      rs2 = Locmap.setpair (loc_result (ef_sig ef)) res rs1 ->
-      step (Callstate s (External ef) rs1 m (*SACC:*)sz)
+      rs2 = Locmap.setpair (loc_result (ef_sig ef)) res (undef_regs destroyed_at_call rs1) ->
+      step (Callstate s (External ef) rs1 m sz)
          t (Returnstate s rs2 m')
   | exec_return:
-      forall s f sp rs0 c rs m (*SACC:*)m',
-  (*SACC:*)Mem.unrecord_stack_block m = Some m' ->
+      forall s f sp rs0 c rs m m',
+        Mem.unrecord_stack_block m = Some m' ->
       step (Returnstate (Stackframe f sp rs0 c :: s) rs m)
         E0 (State s f sp c rs m').
+
+Variable init_m: mem.
+
+Inductive bounds_stack (m: mem) : list stackframe -> Prop :=
+| bs_nil: bounds_stack m nil
+| bs_cons f sp ls c cs
+    (VB: Mem.valid_block m sp)
+    (PERM: forall ofs p,
+        Mem.perm m sp ofs Max p ->
+        0 <= ofs < fn_stacksize f)
+    (BS: bounds_stack m cs):
+    bounds_stack m (Stackframe f (Vptr sp Ptrofs.zero) ls c :: cs).
+
+Inductive nextblock_properties_linear: state -> Prop :=
+| nextblock_properties_linear_intro:
+    forall cs f sp c ls m 
+      (INIT_VB: Ple (Mem.nextblock init_m) (Mem.nextblock m))
+      (PERM_stack: forall (ofs : Z) (p : permission), Mem.perm m sp ofs Max p -> 0 <= ofs < fn_stacksize f)
+      (BS: bounds_stack m cs)
+      (VB: Mem.valid_block m sp),
+      nextblock_properties_linear (State cs f (Vptr sp Ptrofs.zero) c ls m)
+| nextblock_properties_linear_call:
+    forall  cs f ls m sz
+       (INIT_VB: Ple (Mem.nextblock init_m) (Mem.nextblock m))
+       (BS: bounds_stack m cs),
+      nextblock_properties_linear (Callstate cs f ls m sz)
+| nextblock_properties_linear_return:
+    forall cs ls m 
+      (INIT_VB: Ple (Mem.nextblock init_m) (Mem.nextblock m))
+      (BS: bounds_stack m cs),
+      nextblock_properties_linear (Returnstate cs ls m).
+
+
+Lemma bounds_stack_perm:
+  forall s m (BS: bounds_stack m s)
+    m' (PERM: forall b ofs p, Mem.valid_block m b -> Mem.perm m' b ofs Max p -> Mem.perm m b ofs Max p)
+    (PLE: Ple (Mem.nextblock m) (Mem.nextblock m')),
+    bounds_stack m' s.
+Proof.
+  induction s; simpl; intros; eauto.
+  constructor.
+  inv BS. constructor; eauto.
+  unfold Mem.valid_block in *; xomega.
+Qed.
+
+Lemma bounds_stack_store:
+  forall s m (BS: bounds_stack m s)
+    chunk b o v m'
+    (STORE: Mem.store chunk m b o v = Some m'),
+    bounds_stack m' s.
+Proof.
+  intros; eapply bounds_stack_perm; eauto.
+  intros. eapply Mem.perm_store_2; eauto.
+  erewrite <- Mem.nextblock_store; eauto. xomega.
+Qed.
+
+Lemma bounds_stack_free:
+  forall s m (BS: bounds_stack m s)
+    b lo hi m'
+    (FREE: Mem.free m b lo hi = Some m'),
+    bounds_stack m' s.
+Proof.
+  intros.
+  eapply bounds_stack_perm; eauto.
+  intros; eapply Mem.perm_free_3; eauto.
+  intros; erewrite <- Mem.nextblock_free; eauto. xomega.
+Qed.
+
+
+Lemma bounds_stack_unrecord_stack_block:
+  forall s m (BS: bounds_stack m s)
+    m'
+    (FREE: Mem.unrecord_stack_block m = Some m'),
+    bounds_stack m' s.
+Proof.
+  intros.
+  generalize (Mem.unrecord_stack_block_mem_unchanged _ _ FREE);
+    let A := fresh in
+    intro A; decompose [and] A; clear A;
+      generalize (fun b => Mem.unrecord_stack_block_get_frame_info _ _ b FREE).
+  intros; eapply bounds_stack_perm; eauto.
+  intros. eapply H2; eauto.
+  rewrite H0; xomega.
+Qed.
+
+Lemma bounds_stack_record_stack_block:
+  forall s m (BS: bounds_stack m s)
+    m' b
+    (FREE: Mem.record_stack_blocks m b = Some m'),
+    bounds_stack m' s.
+Proof.
+  intros.
+  generalize (Mem.record_stack_blocks_mem_unchanged _ _ _ FREE);
+    let A := fresh in
+    intro A; decompose [and] A; clear A.
+  intros; eapply bounds_stack_perm; eauto.
+  intros. eapply H2; eauto.
+  rewrite H0; xomega.
+Qed.
+
+
+Lemma bounds_stack_push:
+  forall s m (BS: bounds_stack m s),
+    bounds_stack (Mem.push_new_stage m) s.
+Proof.
+  intros.
+  eapply bounds_stack_perm; eauto.
+  intros. rewrite Mem.push_new_stage_perm in H0. auto.
+  rewnb. xomega.
+Qed.
+
+Theorem np_linear_step:
+  forall s1 t s2,
+    step s1 t s2 ->
+    nextblock_properties_linear s1 ->
+    nextblock_properties_linear s2.
+Proof.
+  destruct 1; simpl; intros NPL; inv NPL; try econstructor; unfold Mem.valid_block; rewnb; eauto.
+  intros ofs p P. eapply PERM_stack. eapply Mem.storev_perm_inv; eauto.
+  destruct a; simpl in *; try discriminate.
+  eapply bounds_stack_store; eauto.
+  apply bounds_stack_push.
+  constructor; auto.
+  eapply bounds_stack_perm.
+  eapply bounds_stack_free; eauto.
+  intros b0 ofs p VB2; repeat rewrite_perms. tauto.
+  rewnb. xomega.
+  intros; eapply PERM_stack. eapply Mem.unrecord_stack_block_perm in H2. 2: eauto.
+  eapply external_call_max_perm in H2. 2: eauto.
+  rewrite Mem.push_new_stage_perm in H2. eauto.
+  red; rewnb; auto.
+  eapply bounds_stack_unrecord_stack_block. 2: eauto.
+  eapply bounds_stack_perm. apply bounds_stack_push. eauto.
+  intros. eapply external_call_max_perm; eauto.
+  rewnb; xomega.
+  eapply bounds_stack_free; eauto.
+  xomega.
+  intros.
+  eapply Mem.record_stack_block_perm in H1. 2: eauto.
+  eapply Mem.perm_alloc_3; eauto.
+  eapply bounds_stack_record_stack_block. 2: eauto.
+  eapply bounds_stack_perm; eauto.
+  intros. eapply Mem.perm_alloc_inv in H2. 2: eauto.
+  destruct eq_block; auto. subst. eapply Mem.fresh_block_alloc in H1; eauto. easy.
+  rewnb; xomega.
+  exploit Mem.alloc_result; eauto. intro; subst. xomega.
+  eapply bounds_stack_perm; eauto.
+  intros; eapply external_call_max_perm; eauto.
+  rewnb. xomega.
+  inv BS. constructor; unfold Mem.valid_block; rewnb; eauto; try xomega.
+  intros; eapply PERM. eapply Mem.unrecord_stack_block_perm in H0; eauto.
+  eapply bounds_stack_unrecord_stack_block; eauto.
+Qed.
 
 End RELSEM.
 
 Inductive initial_state (p: program): state -> Prop :=
-  | initial_state_intro: forall b f m0 (*SACC:*)m2,
+  | initial_state_intro: forall b f m0 m2,
       let ge := Genv.globalenv p in
       Genv.init_mem p = Some m0 ->
       Genv.find_symbol ge p.(prog_main) = Some b ->
       Genv.find_funct_ptr ge b = Some f ->
       funsig f = signature_main ->
-  (*SACC:*)Mem.record_init_sp m0 = Some m2 ->
-      initial_state p (Callstate nil f (Locmap.init Vundef) ((*SACC:*)Mem.push_new_stage m2) ((*SACC:*)fn_stack_requirements (prog_main p))).
+      Mem.record_init_sp m0 = Some m2 ->
+      initial_state p (Callstate nil f (Locmap.init Vundef) (Mem.push_new_stage m2) (fn_stack_requirements (prog_main p))).
 
 Inductive final_state: state -> int -> Prop :=
   | final_state_intro: forall rs m retcode,
@@ -285,6 +437,6 @@ Inductive final_state: state -> int -> Prop :=
       final_state (Returnstate nil rs m) retcode.
 
 Definition semantics (p: program) :=
-  Semantics step (initial_state p) final_state (Genv.globalenv p).
+  Semantics (step (Locmap.init Vundef)) (initial_state p) final_state (Genv.globalenv p).
 
-End STACK_WRAPPER.
+End WITHEXTERNALCALLSOPS.
